src/reorder/Reorder.v
@@ -1,3 +1,4 @@
+Require Import Basics.
 Require Import Bool.
 Require Import List.
 Require Import ProofIrrelevance.
@@ -6,30 +7,18 @@ Require Import sflib.
 
 Require Import Basic.
 Require Import Event.
-Require Import Syntax.
-Require Import Semantics.
-Require Import Thread.
+Require Import Program.
 Require Import Memory.
 Require Import Configuration.
-Require Import Program.
 Require Import Simulation.
+Require Import Syntax.
+Require Import Semantics.
 
 Set Implicit Arguments.
 
 (* TODO: now supporting only the reordering of load and store *)
 
-Definition reorderable_message (msg1 msg2:Message.t): bool :=
-  match msg1, msg2 with
-  | Message.rw (RWEvent.read l1 c1 o1) t1,
-    Message.rw (RWEvent.write l2 c2 o2) t2 =>
-    (negb (Loc.eqb l1 l2)) &&
-    (negb (Ordering.ord Ordering.acquire o1)) &&
-    (negb (Ordering.ord Ordering.release o2))
-  | _, _ =>
-    false
-  end.
-
-Definition reorderable_instr (i1 i2:Instr.t): bool :=
+Definition reordered_instr (i1 i2:Instr.t): bool :=
   match i1, i2 with
   | Instr.load r1 l1 o1,
     Instr.store l2 v2 o2 =>
@@ -41,251 +30,223 @@ Definition reorderable_instr (i1 i2:Instr.t): bool :=
     false
   end.
 
-Inductive trans_stmt: forall (s1 s2:Stmt.t), Prop :=
-| trans_stmt_instr i:
-    trans_stmt
+Inductive reordered_stmt: forall (s1 s2:Stmt.t), Prop :=
+| reordered_stmt_instr i:
+    reordered_stmt
       (Stmt.instr i)
       (Stmt.instr i)
-| trans_stmt_ite
+| reordered_stmt_ite
     cond c11 c12 c21 c22
-    (TRANS1: trans_stmts c11 c21)
-    (TRANS2: trans_stmts c12 c22):
-    trans_stmt
+    (REORDER1: reordered_stmts c11 c21)
+    (REORDER2: reordered_stmts c12 c22):
+    reordered_stmt
       (Stmt.ite cond c11 c12)
       (Stmt.ite cond c21 c22)
-| trans_stmt_dowhile
+| reordered_stmt_dowhile
     cond c1 c2
-    (TRANS2: trans_stmts c1 c2):
-    trans_stmt
+    (REORDER2: reordered_stmts c1 c2):
+    reordered_stmt
       (Stmt.dowhile c1 cond)
       (Stmt.dowhile c2 cond)
 
-with trans_stmts: forall (s1 s2:list Stmt.t), Prop :=
-| trans_stmts_nil:
-    trans_stmts nil nil
-| trans_stmts_cons
+with reordered_stmts: forall (s1 s2:list Stmt.t), Prop :=
+| reordered_stmts_nil:
+    reordered_stmts nil nil
+| reordered_stmts_cons
     s11 s12 s21 s22
-    (TRANS1: trans_stmt s11 s21)
-    (TRANS2: trans_stmts s12 s22):
-    trans_stmts (s11::s12) (s21::s22)
-| trans_stmts_reorder
+    (REORDER1: reordered_stmt s11 s21)
+    (REORDER2: reordered_stmts s12 s22):
+    reordered_stmts (s11::s12) (s21::s22)
+| reordered_stmts_reorder
     i1 i2 s1 s2
-    (REORDER: reorderable_instr i1 i2)
-    (TRANS: trans_stmts s1 s2):
-    trans_stmts
+    (REORDER: reordered_instr i1 i2)
+    (REORDER: reordered_stmts s1 s2):
+    reordered_stmts
       ((Stmt.instr i1)::(Stmt.instr i2)::s1)
       ((Stmt.instr i2)::(Stmt.instr i1)::s2)
 .
 
-Scheme trans_stmt_ind_ := Induction for trans_stmt Sort Prop
-with trans_stmts_ind_ := Induction for trans_stmts Sort Prop.
-Combined Scheme trans_ind from trans_stmt_ind_, trans_stmts_ind_.
+Scheme reordered_stmt_ind_ := Induction for reordered_stmt Sort Prop
+with reordered_stmts_ind_ := Induction for reordered_stmts Sort Prop.
+Combined Scheme reordered_ind from reordered_stmt_ind_, reordered_stmts_ind_.
 
-Inductive trans_prog_thread: forall (text1 text2:Program.thread_t), Prop :=
-| trans_prog_thread_intro
+Inductive reordered_thread: forall (text1 text2:Thread.syntax), Prop :=
+| reordered_thread_intro
     s1 s2
-    (TRANS: trans_stmts s1 s2):
-    trans_prog_thread
-      (Program.thread_mk lang s1)
-      (Program.thread_mk lang s2)
+    (REORDER: reordered_stmts s1 s2):
+    reordered_thread
+      (Thread.mk_syntax lang s1)
+      (Thread.mk_syntax lang s2)
 .
 
-Inductive trans_prog (prog1 prog2:Program.t): Prop :=
-| trans_prog_intro
-    (TRANS: IdentMap.rel2 trans_prog_thread prog1 prog2)
+Inductive reordered_program i: forall (prog1 prog2:Program.syntax), Prop :=
+| reordered_program_intro
+    prog1 th1 th2
+    (TH1: IdentMap.find i prog1 = Some th1)
+    (REORDER: reordered_thread th1 th2):
+    reordered_program i prog1 (IdentMap.add i th2 prog1)
 .
 
-Inductive consumed (i2:Instr.t): forall (c1 c2:list Stmt.t), Prop :=
-| consumed_intro
+Inductive consumed_stmts (i2:Instr.t): forall (c1 c2:list Stmt.t), Prop :=
+| consumed_stmts_intro
     i1 c1 c2
-    (REORDER: reorderable_instr i1 i2)
-    (TRANS: trans_stmts c1 c2):
-    consumed i2 ((Stmt.instr i1)::(Stmt.instr i2)::c1) ((Stmt.instr i1)::c2)
+    (REORDER: reordered_instr i1 i2)
+    (REORDER: reordered_stmts c1 c2):
+    consumed_stmts i2 ((Stmt.instr i1)::(Stmt.instr i2)::c1) ((Stmt.instr i1)::c2)
 .
 
-Inductive sim_thread: forall (e:option ThreadEvent.t) (th1 th2:Thread.t), Prop :=
-| sim_thread_trans
+Inductive consumed_thread i: forall (text1 text2:Thread.syntax), Prop :=
+| consumed_thread_intro
+    s1 s2
+    (CONSUME: consumed_stmts i s1 s2):
+    consumed_thread
+      i
+      (Thread.mk_syntax lang s1)
+      (Thread.mk_syntax lang s2)
+.
+
+Inductive sim_thread: forall (th1 th2:Thread.t), Prop :=
+| sim_thread_intro
     rs s1 s2
-    (TRANS: trans_stmts s1 s2):
+    (REORDER: reordered_stmts s1 s2):
     sim_thread
-      None
       (Thread.mk lang (State.mk rs s1))
       (Thread.mk lang (State.mk rs s2))
-| sim_thread_consumed
-    rs1 rs2 s1 s2 i e
-    (CONSUMED: consumed i s1 s2)
-    (EVAL: RegFile.eval_instr rs1 i e rs2):
-    sim_thread
+.
+
+Inductive sim_consumed_thread (e:option RWEvent.t): forall (th1 th2:Thread.t), Prop :=
+| sim_consumed_thread_intro
+    rs1 rs2 s1 s2 i
+    (CONSUMED: consumed_stmts i s1 s2)
+    (EVAL: RegFile.eval_instr rs1 i (option_map (compose ThreadEvent.mem ThreadEvent.rw) e) rs2):
+    sim_consumed_thread
       e
       (Thread.mk lang (State.mk rs1 s1))
       (Thread.mk lang (State.mk rs2 s2))
 .
 
-Inductive sim_history: forall (b1 b2:list Message.t), Prop :=
-| sim_history_nil:
-    sim_history nil nil
-| sim_history_cons
+Definition sim_message (msg1 msg2:Message.t): bool :=
+  match msg1, msg2 with
+  | Message.rw (RWEvent.read l1 c1 o1) t1,
+    Message.rw (RWEvent.write l2 c2 o2) t2 =>
+    (negb (Loc.eqb l1 l2)) &&
+    (negb (Ordering.ord Ordering.acquire o1)) &&
+    (negb (Ordering.ord Ordering.release o2))
+  | _, _ =>
+    false
+  end.
+
+Inductive sim_buffer: forall (b1 b2:Buffer.t), Prop :=
+| sim_buffer_nil:
+    sim_buffer nil nil
+| sim_buffer_cons
     msg b1 b2
-    (HISTORY: sim_history b1 b2):
-    sim_history (b1 ++ [msg]) (b2 ++ [msg])
-| sim_history_reorder
+    (BUFFER: sim_buffer b1 b2):
+    sim_buffer (b1 ++ [msg]) (b2 ++ [msg])
+| sim_buffer_reorder
     msg1 msg2 b1 b2
-    (MSG: reorderable_message msg1 msg2)
-    (HISTORY: sim_history b1 b2):
-    sim_history (b1 ++ [msg1; msg2]) (b2 ++ [msg2; msg1])
+    (MSG: sim_message msg1 msg2)
+    (BUFFER: sim_buffer b1 b2):
+    sim_buffer (b1 ++ [msg1; msg2]) (b2 ++ [msg2; msg1])
 .
 
-Inductive sim_buffer: forall (e:option ThreadEvent.t) (b1 b2:Buffer.t), Prop :=
-| sim_buffer_trans
-    history1 history2 inception
-    (HISTORY: sim_history history1 history2):
-    sim_buffer
-      None
-      (Buffer.mk history1 inception)
-      (Buffer.mk history2 inception)
-| sim_buffer_consumed_observable
-    msg history1 history2 inception2
-    (HISTORY: sim_history history1 history2)
-    (OBSERVABLE: Message.observable msg):
-    sim_buffer
-      (Some (Message.get_threadevent msg))
-      (Buffer.mk history1 (MessageSet.add msg inception2))
-      (Buffer.mk (history2 ++ [msg]) inception2)
-| sim_buffer_consumed_unobservable
-    msg history1 history2 inception
-    (HISTORY: sim_history history1 history2)
-    (UNOBSERVABLE: ~ Message.observable msg):
-    sim_buffer
-      (Some (Message.get_threadevent msg))
-      (Buffer.mk history1 inception)
-      (Buffer.mk (history2 ++ [msg]) inception)
+Inductive sim_consumed_buffer: forall (e:option (RWEvent.t * nat)) (b1 b2:Buffer.t), Prop :=
+| sim_consumed_buffer_None
+    b1 b2
+    (BUFFER: sim_buffer b1 b2):
+    sim_consumed_buffer None b1 b2
+| sim_consumed_buffer_Some
+    e ts b1 b2
+    (BUFFER: sim_buffer b1 b2):
+    sim_consumed_buffer (Some (e, ts)) b1 (b2 ++ [Message.rw e ts])
 .
 
-Inductive sim_thread_buffer: forall (th1 th2:option Thread.t) (b1 b2:option Buffer.t), Prop :=
-| sim_thread_buffer_None:
-    sim_thread_buffer None None None None
-| sim_thread_buffer_Some
-    th1 th2 b1 b2 e
-    (THREAD: sim_thread e th1 th2)
-    (BUFFER: sim_buffer e b1 b2):
-    sim_thread_buffer (Some th1) (Some th2) (Some b1) (Some b2)
+Inductive sim_inceptions i: forall (e:option (RWEvent.t * nat)) (inceptions1 inceptions2:InceptionSet.t), Prop :=
+| sim_inceptions_None inceptions:
+    sim_inceptions i None inceptions inceptions
+| sim_inceptions_Some
+    e ts inceptions2:
+    sim_inceptions
+      i (Some (e, ts))
+      (InceptionSet.add (Inception.mk (Message.rw e ts) (IdentSet.singleton i)) inceptions2)
+      inceptions2
 .
 
-Definition sim_threads_memory (th1 th2:Threads.t) (m1 m2:Memory.t): Prop :=
-  forall i,
-    <<SIM: sim_thread_buffer
-             (IdentMap.find i th1) (IdentMap.find i th2)
-             (IdentMap.find i m1) (IdentMap.find i m2)>>.
-
-Inductive sim_configuration (c1 c2:Configuration.t): Prop :=
-| sim_configuration_intro
-    (CLOCKS: Clocks.le c1.(Configuration.clocks) c2.(Configuration.clocks))
-    (CUR: sim_threads_memory
-            c1.(Configuration.threads) c2.(Configuration.threads)
-            c1.(Configuration.memory) c2.(Configuration.memory))
-    (STACK:
-       Forall2
-         (fun stk1 stk2 => sim_threads_memory stk1.(fst) stk2.(fst) stk1.(snd) stk2.(snd))
-         c1.(Configuration.stack) c2.(Configuration.stack))
+Inductive sim_configuration: forall (conf1 conf2:Configuration.t), Prop :=
+| sim_configuration_reordered
+    i c1 c2 p1 p2 bs1 bs2 inceptions1 inceptions2
+    th1 th2 b1 b2
+    (THREAD1: IdentMap.find i p1 = Some th1)
+    (BUFFER1: IdentMap.find i bs1 = Some b1)
+    (THREAD2: sim_thread th1 th2)
+    (BUFFER2: sim_buffer b1 b2)
+    (CLOCKS: c1 = c2)
+    (PROGRAMS: p2 = IdentMap.add i th2 p1)
+    (BUFFERS: bs2 = IdentMap.add i b2 bs1)
+    (INCEPTIONS: inceptions1 = inceptions2):
+    sim_configuration
+      (Configuration.mk c1 p1 (Memory.mk bs1 inceptions1))
+      (Configuration.mk c2 p2 (Memory.mk bs2 inceptions2))
+| sim_configuration_consumed
+    i e c1 c2 p1 p2 bs1 bs2 inceptions1 inceptions2
+    th1 th2 b1 b2
+    (CLOCKS: Clocks.le c1 c2)
+    (THREAD1: IdentMap.find i p1 = Some th1)
+    (BUFFER1: IdentMap.find i bs1 = Some b1)
+    (THREAD2: sim_consumed_thread (option_map fst e) th1 th2)
+    (BUFFER2: sim_consumed_buffer e b1 b2)
+    (PROGRAMS: p2 = IdentMap.add i th2 p1)
+    (BUFFERS: bs2 = IdentMap.add i b2 bs1)
+    (INCEPTIONS: sim_inceptions i e inceptions1 inceptions2):
+    sim_configuration
+      (Configuration.mk c1 p1 (Memory.mk bs1 inceptions1))
+      (Configuration.mk c2 p1 (Memory.mk bs2 inceptions2))
 .
-
-Lemma sim_load_thread
-      text_src text_tgt th_tgt
-      (TRANS: trans_prog_thread text_src text_tgt)
-      (TGT: Program.load_thread text_tgt th_tgt):
-  exists th_src,
-    <<SRC: Program.load_thread text_src th_src>> /\
-    <<SIM: sim_thread None th_src th_tgt>>.
-Proof.
-  inv TRANS; inv TGT.
-  apply inj_pair2 in H1. subst.
-  inv LOAD. exists (Thread.mk lang (State.mk RegFile.init s1)).
-  split; repeat constructor; auto.
-Qed.
 
 Lemma sim_load
-      prog_src prog_tgt
-      (TRANS: trans_prog prog_src prog_tgt):
+      i prog_src prog_tgt
+      (REORDER: reordered_program i prog_src prog_tgt):
   Simulation.LOAD prog_src prog_tgt sim_configuration.
 Proof.
-  inv TRANS.
-  ii. inv TGT. inv LOAD.
-  generalize (IdentMap.rel2_elim TRANS0 LOAD0). intro REL2.
-  eapply (IdentMap.rel2_implies
-            (fun text th => exists th', Program.load_thread text th' /\
-                                sim_thread None th' th))
-    in REL2.
-  all: cycle 1.
-  { intros. des. inv H. inv H0. inv LOAD.
-    apply inj_pair2 in H2. subst.
-    repeat econs; eauto.
-  }
-
-  apply IdentMap.rel2_intro in REL2. des.
-  eexists (Configuration.mk Clocks.init mb _ []).
-  repeat econs; simpl; eauto.
-  intro i. rewrite ? IdentMap.Facts.map_o.
-  specialize (BC i). inv BC; simpl; try constructor.
-  repeat econs; eauto.
+  inv REORDER. econs 1; eauto.
+  - unfold Program.load.
+    rewrite IdentMap.Facts.map_o, TH1.
+    simpl. eauto.
+  - rewrite IdentMap.Facts.map_o, TH1.
+    simpl. eauto.
+  - instantiate (1 := Thread.load th2).
+    inv REORDER0. econs. auto.
+  - econs.
+  - apply IdentMap.map_add.
+  - apply IdentMap.map_add.
 Qed.
 
 Lemma sim_step: Simulation.STEP sim_configuration.
 Proof.
-  ii. inv STEP.
-  - admit.
-  - destruct src. inv SIM. simpl in *.
-    eexists. split.
-    + eapply srcsteps_progress.
-      { apply tausteps_nil. }
-      apply Configuration.step_dream.
-    + econs; simpl; auto.
-  - admit.
-  - destruct src. inv SIM. inv STACK. simpl in *. subst.
-    eexists. split.
-    + eapply srcsteps_progress.
-      { apply tausteps_nil. }
-      apply Configuration.step_commit.
-      * admit.
-      * admit.
-    + econs; simpl; eauto.
-  - destruct src. inv SIM. inv STACK. simpl in *. subst.
-    eexists. split.
-    + eapply srcsteps_progress.
-      { apply tausteps_nil. }
-      eapply Configuration.step_syscall.
-      admit.
-    + econs; simpl; eauto.
-      admit.
-Admitted.
-
-Lemma sim_observable: Simulation.OBSERVABLE sim_configuration.
-Proof.
-  (* TODO: bogus step for *each* thread *)
 Admitted.
 
 Lemma sim_terminal: Simulation.TERMINAL sim_configuration.
 Proof.
-  ii. destruct src, tgt. inv SIM. inv TERM.
-  simpl in *. subst. inv STACK.
-  eexists. split.
+  ii. eexists. split.
   { apply tausteps_nil. }
-  econs; simpl; eauto.
-  econs. ii. specialize (CUR i). inv CUR; try congruence.
-  rewrite THREAD in H0. inv H0.
-  inv THREADS. symmetry in H. specialize (TERMINAL _ _ H).
-  inv THREAD0.
-  - inv TERMINAL. simpl in *. subst.
-    inv TRANS. econs.
-  - inv TERMINAL. simpl in *. subst.
-    inv CONSUMED.
+  econs. econs. intros.
+  inv TERM. inv PROGRAM. specialize (TERMINAL i).
+  inv SIM; simpl in *.
+  - rewrite IdentMap.Facts.add_o in *.
+    destruct (IdentMap.Properties.F.eq_dec i0 i).
+    + exploit TERMINAL; eauto. intro X.
+      inv THREAD2. inv X. simpl in *. subst.
+      inv REORDER. rewrite THREAD in THREAD1. inv THREAD1. auto.
+    + apply TERMINAL. auto.
+  - apply TERMINAL. auto.
 Qed.
 
 Definition sim
-           prog_src prog_tgt
-           (TRANS: trans_prog prog_src prog_tgt):
+           i prog_src prog_tgt
+           (REORDER: reordered_program i prog_src prog_tgt):
   Simulation.t prog_src prog_tgt :=
   Simulation.mk
-    (sim_load TRANS)
+    _ _
+    (sim_load REORDER)
     sim_step
-    sim_observable
     sim_terminal.
