src/while/Semantics.v
@@ -1,7 +1,7 @@
 Require Import List.
 Require Import Event.
 Require Import Syntax.
-Require Import Thread.
+Require Import Program.
 
 Set Implicit Arguments.
 
@@ -29,21 +29,21 @@ Module RegFile.
       eval_instr
         rf
         (Instr.load lhs rhs ord)
-        (Some (ThreadEvent.rw (RWEvent.read rhs val ord)))
+        (Some (ThreadEvent.mem (ThreadEvent.rw (RWEvent.read rhs val ord))))
         (RegFun.add lhs val rf)
   | eval_store
       rf lhs rhs ord:
       eval_instr
         rf
         (Instr.store lhs rhs ord)
-        (Some (ThreadEvent.rw (RWEvent.write lhs (eval_value rf rhs) ord)))
+        (Some (ThreadEvent.mem (ThreadEvent.rw (RWEvent.write lhs (eval_value rf rhs) ord))))
         rf
   | eval_fetch_add
       rf lhs loc addendum ord val:
       eval_instr
         rf
         (Instr.fetch_add lhs loc addendum ord)
-        (Some (ThreadEvent.rw (RWEvent.update loc val (Const.add val (eval_value rf addendum)) ord)))
+        (Some (ThreadEvent.mem (ThreadEvent.rw (RWEvent.update loc val (Const.add val (eval_value rf addendum)) ord))))
         (RegFun.add lhs val rf)
   | eval_assign
       rf lhs rhs:
@@ -57,7 +57,7 @@ Module RegFile.
       eval_instr
         rf
         (Instr.fence ord)
-        (Some (ThreadEvent.fence ord))
+        (Some (ThreadEvent.mem (ThreadEvent.fence ord)))
         rf
   | eval_syscall
       rf lhs rhses lhs_val:
@@ -75,10 +75,8 @@ Module State.
     stmts: list Stmt.t;
   }.
 
-  Inductive load: forall (text:list Stmt.t) (s:t), Prop :=
-  | load_intro text:
-      load text (mk RegFile.init text)
-  .
+  Definition load (text:list Stmt.t): t :=
+    mk RegFile.init text.
 
   Definition is_terminal (s:t): Prop :=
     stmts s = nil.
