src/lang/Configuration.v
@@ -1,0 +1,102 @@
+Require Import sflib.
+
+Require Import Basic.
+Require Import Event.
+Require Import Program.
+Require Import Memory.
+
+Set Implicit Arguments.
+
+Module Configuration.
+  Structure t := mk {
+    clocks: Clocks.t;
+    program: Program.t;
+    memory: Memory.t;
+  }.
+
+  Definition load (s:Program.syntax): Configuration.t :=
+    Configuration.mk
+      Clocks.init
+      (Program.load s)
+      (Memory.init s).
+
+  Inductive is_terminal (c:t): Prop :=
+  | is_terminal_intro
+      (PROGRAM: Program.is_terminal c.(program))
+  .
+
+  Inductive internal_step: forall (c1:t) (c2:t), Prop :=
+  | step_tau
+      c th1 th2 i m
+      (PROGRAM: Program.step th1 i None th2):
+      internal_step (mk c th1 m) (mk c th2 m)
+  | step_mem
+      i e
+      c th1 th2 m1 m2
+      (PROGRAM: Program.step th1 i (Some (ThreadEvent.mem e)) th2)
+      (MEMORY: Memory.step c m1 i e m2)
+      (CONSISTENT: Memory.consistent m2):
+      internal_step (mk c th1 m1) (mk c th2 m2)
+  | step_inception
+      c th m1 m2 event ts loc val i n ths
+      (STEPS: internal_steps (mk c th m1) (mk c th m2))
+      (INCEPTIONS: InceptionSet.Empty m2.(Memory.inceptions))
+      (WRITING: RWEvent.is_writing event = Some (loc, val))
+      (UPDATE:
+         forall loc valr valw ord (EVENT: event = RWEvent.update loc valr valw ord),
+         exists event0 ts0 pos0 val0,
+           <<IN0: Memory.In m1 (Message.rw event0 ts0) pos0>> /\
+           <<TS0: ts0 + 1 = ts>> /\
+           <<EVENT0: RWEvent.is_writing event0 = Some (loc, val0)>>)
+      (MESSAGE: Memory.In m2 (Message.rw event ts) (Memory.Position.buffer i n))
+      (PROGRAM: IdentSet.mem i ths):
+      internal_step (mk c th m1)
+                    (mk c th (Memory.mk m1.(Memory.buffers) (InceptionSet.add (Inception.mk (Message.rw event ts) ths) m1.(Memory.inceptions))))
+  | step_confirm
+      c th1 th2 m1 inceptions2
+      i e ts ths b
+      (PROGRAM: Program.step th1 i (Some (ThreadEvent.mem (ThreadEvent.rw e))) th2)
+      (INCEPTIONS: InceptionSet.remove_if_exists (Inception.mk (Message.rw e ts) ths) m1.(Memory.inceptions) = Some inceptions2)
+      (THS: IdentSet.mem i ths)
+      (BUFFER: IdentMap.find i c.(memory).(Memory.buffers) = Some b):
+      internal_step c
+                    (mk c.(clocks) c.(program)
+                        (Memory.mk (IdentMap.add i (b ++ [Message.rw e ts]) c.(memory).(Memory.buffers)) inceptions2))
+
+  with internal_steps: forall (c1 c2:t), Prop :=
+  | steps_nil c:
+      internal_steps c c
+  | steps_cons
+      c1 c2 c3
+      (STEP: internal_step c1 c2)
+      (STEPS: internal_steps c2 c3):
+      internal_steps c1 c3
+  .
+
+  Inductive feasible (c:t): Prop :=
+  | feasible_intro
+      c'
+      (STEP: internal_steps c c')
+      (INCEPTIONS: InceptionSet.Empty c'.(memory).(Memory.inceptions))
+  .
+
+  Inductive step: forall (c1:t) (e:option Event.t) (c2:t), Prop :=
+  | step_internal
+      c1 c2
+      (STEP: internal_step c1 c2)
+      (FEASIBLE: feasible c2):
+      step c1 None c2
+  | step_commit
+      c1 th m c2
+      (MEMORY: InceptionSet.Empty m.(Memory.inceptions))
+      (CLOCKS: Clocks.le c1 c2)
+      (CONSISTENT: Memory.consistent m)
+      (FEASIBLE: feasible (mk c2 th m)):
+      step (mk c1 th m) None (mk c2 th m)
+  | step_syscall
+      c th1 m i e th2
+      (PROGRAM: Program.step th1 i (Some (ThreadEvent.syscall e)) th2)
+      (FEASIBLE: feasible (mk c th2 m)):
+      step (mk c th1 m) (Some e) (mk c th2 m)
+  .
+End Configuration.
