src/lang/Event.v
@@ -1,0 +1,208 @@
+Require Import List.
+Require Import PeanoNat.
+Require Import Orders.
+Require Import MSetList.
+Require Import Omega.
+
+Require Import sflib.
+
+Require Import Basic.
+Require Import BoolOrderedType.
+
+Set Implicit Arguments.
+Import ListNotations.
+
+
+Module Loc := Ident.
+Module LocSet := IdentSet.
+Module LocMap := IdentMap.
+Module LocFun := IdentFun.
+
+
+Module Const <: OrderedTypeWithLeibniz.
+  Include Nat.
+
+  Lemma eq_leibniz (x y: t): eq x y -> x = y.
+  Proof. auto. Qed.
+  
+  Ltac ltb_tac :=
+    match goal with
+    | [H: compare ?x1 ?x2 = _ |- _] =>
+      generalize (compare_spec x1 x2); rewrite H; clear H;
+      intro H; inversion H; subst; clear H
+    | [H: lt ?x ?x |- _] =>
+      destruct lt_strorder; congruence
+    | [H: lt ?x ?y |- _] =>
+      rewrite H in *; clear H
+    | [H: eq ?x ?y |- _] =>
+      rewrite H in *; clear H
+    end.
+End Const.
+
+
+Module Ordering <: OrderedTypeWithLeibniz.
+  Module Raw <: BoolOrderedType.S.
+    Inductive t_ :=
+    | relaxed
+    | acquire
+    | release
+    | relacq
+    .
+    Definition t := t_.
+
+    Definition eq_dec (x y:t): {x = y} + {x <> y}.
+    Proof. decide equality. Qed.
+
+    Definition ltb (lhs rhs:t): bool :=
+      match lhs, rhs with
+      | relaxed, relaxed => false
+      | relaxed, _ => true
+      | acquire, relaxed => false
+      | acquire, acquire => false
+      | acquire, _ => true
+      | release, relaxed => false
+      | release, acquire => false
+      | release, release => false
+      | release, _ => true
+      | relacq, _ => false
+      end.
+
+    Lemma ltb_trans (x y z:t) (XY: ltb x y) (YZ: ltb y z): ltb x z.
+    Proof. repeat intro. destruct x, y, z; auto. Qed.
+
+    Lemma ltb_irrefl x: ~ ltb x x.
+    Proof. repeat intro. destruct x; auto. Qed.
+
+    Lemma ltb_eq (lhs rhs:t) (LR: ~ ltb lhs rhs) (RL: ~ ltb rhs lhs): lhs = rhs.
+    Proof. repeat intro. destruct lhs, rhs; simpl in *; congruence. Qed.
+  End Raw.
+
+  Include Raw <+ BoolOrderedType.Make (Raw).
+
+  Definition ord (lhs rhs:t): bool :=
+    match lhs, rhs with
+    | acquire, relaxed => false
+    | acquire, release => false
+    | release, relaxed => false
+    | release, acquire => false
+    | _, _ => true
+    end.
+End Ordering.
+
+
+Module RWEvent <: OrderedTypeWithLeibniz.
+  Module Raw <: BoolOrderedType.S.
+    Inductive t_ :=
+    | read (loc:Loc.t) (val:Const.t) (ord:Ordering.t)
+    | write (loc:Loc.t) (val:Const.t) (ord:Ordering.t)
+    | update (loc:Loc.t) (rval wval:Const.t) (ord:Ordering.t)
+    .
+    Definition t := t_.
+
+    Definition eq_dec (x y:t): {x = y} + {x <> y}.
+    Proof.
+      decide equality;
+        (try apply Loc.eq_dec);
+        (try apply Const.eq_dec);
+        (try apply Ordering.eq_dec).
+    Qed.
+
+    Definition ltb (lhs rhs:t): bool :=
+      match lhs, rhs with
+      | read l1 v1 o1, read l2 v2 o2 =>
+        compose_comparisons [Loc.compare l1 l2; Const.compare v1 v2; Ordering.compare o1 o2]
+      | write l1 v1 o1, write l2 v2 o2 =>
+        compose_comparisons [Loc.compare l1 l2; Const.compare v1 v2; Ordering.compare o1 o2]
+      | update l1 r1 w1 o1, update l2 r2 w2 o2 =>
+        compose_comparisons [Loc.compare l1 l2; Const.compare r1 r2; Const.compare w1 w2; Ordering.compare o1 o2]
+      | read _ _ _, _ => true
+      | write _ _ _, read _ _ _ => false
+      | write _ _ _, _ => true
+      | update _ _ _ _, _ => false
+      end.
+
+    Lemma ltb_trans (x y z:t) (XY: ltb x y) (YZ: ltb y z): ltb x z.
+    Proof.
+      destruct x, y, z; simpl in *; auto;
+        repeat
+          (try congruence;
+           try omega;
+           try Loc.ltb_tac;
+           try Const.ltb_tac;
+           try Ordering.ltb_tac;
+           try ltb_des).
+    Qed.
+
+    Lemma ltb_irrefl x: ~ ltb x x.
+    Proof.
+      destruct x; simpl in *; auto;
+        repeat
+          (try congruence;
+           try omega;
+           try Loc.ltb_tac;
+           try Const.ltb_tac;
+           try Ordering.ltb_tac;
+           try ltb_des).
+    Qed.
+
+    Lemma ltb_eq (lhs rhs:t) (LR: ~ ltb lhs rhs) (RL: ~ ltb rhs lhs): lhs = rhs.
+    Proof.
+      destruct lhs, rhs; simpl in *; auto;
+        repeat
+          (try congruence;
+           try omega;
+           try Loc.ltb_tac;
+           try Const.ltb_tac;
+           try Ordering.ltb_tac;
+           try ltb_des).
+    Qed.
+  End Raw.
+
+  Include Raw <+ BoolOrderedType.Make (Raw).
+
+  Definition is_writing (e:t): option (Loc.t * Const.t) :=
+    match e with
+    | read _ _ _ => None
+    | write loc val _ => Some (loc, val)
+    | update loc _ val _ => Some (loc, val)
+    end.
+
+  Definition get_ordering (e:t): Ordering.t :=
+    match e with
+    | read _ _ ord => ord
+    | write _ _ ord => ord
+    | update _ _ _ ord => ord
+    end.
+End RWEvent.
+
+
+Module Event.
+  Structure t_ := mk {
+    lhs: Const.t;
+    rhses: list Const.t;
+  }.
+  Definition t := t_.
+
+  Definition eq := @eq t.
+  Program Instance eq_equiv: Equivalence eq.
+  Definition eq_dec (x y:t): {eq x y} + {~ eq x y}.
+  Proof.
+    unfold eq.
+    decide equality;
+      (try apply list_eq_dec);
+      (try apply Const.eq_dec).
+  Qed.
+End Event.
+
+
+Module ThreadEvent.
+  Inductive mem_t :=
+  | rw (e:RWEvent.t)
+  | fence (ord:Ordering.t)
+  .
+
+  Inductive t :=
+  | mem (e:mem_t)
+  | syscall (e:Event.t)
+  .
+End ThreadEvent.
