src/lang/Memory.v
@@ -1,0 +1,400 @@
+Require Import List.
+Require Import Equalities.
+Require Import PeanoNat.
+Require Import Relations.
+Require Import MSetList.
+Require Import Omega.
+
+Require Import sflib.
+Require Import paco.
+
+Require Import DataStructure.
+Require Import Basic.
+Require Import Event.
+Require Import Program.
+Require Import BoolOrderedType.
+
+Set Implicit Arguments.
+Import ListNotations.
+
+Module Clock.
+  Definition t := LocFun.t nat.
+
+  Definition init := LocFun.init 0.
+
+  Definition le (lhs rhs:t): Prop :=
+    forall loc, LocFun.find loc lhs <= LocFun.find loc rhs.
+End Clock.
+
+Module Clocks.
+  Definition t := IdentFun.t Clock.t.
+
+  Definition init := IdentFun.init Clock.init.
+
+  Definition le (lhs rhs:t): Prop :=
+    forall loc, Clock.le (IdentFun.find loc lhs) (IdentFun.find loc rhs).
+End Clocks.
+
+
+Module Message <: OrderedTypeWithLeibniz.
+  Module Raw <: BoolOrderedType.S.
+    Inductive t_ :=
+    | rw (event:RWEvent.t) (timestamp:nat)
+    | fence (ord:Ordering.t)
+    .
+    Definition t := t_.
+
+    Definition eq_dec (x y:t): {x = y} + {x <> y}.
+    Proof.
+      decide equality;
+        (try apply RWEvent.eq_dec);
+        (try apply Nat.eq_dec);
+        (try apply Ordering.eq_dec).
+    Qed.
+
+    Definition ltb (lhs rhs:t): bool :=
+      match lhs, rhs with
+      | rw e1 t1, rw e2 t2 =>
+        compose_comparisons [RWEvent.compare e1 e2; Const.compare t1 t2]
+      | rw _ _, fence _ => true
+      | fence _, rw _ _ => false
+      | fence o1, fence o2 =>
+        compose_comparisons [Ordering.compare o1 o2]
+      end.
+
+    Lemma ltb_trans (x y z:t) (XY: ltb x y) (YZ: ltb y z): ltb x z.
+    Proof.
+      destruct x, y, z; simpl in *; auto;
+        repeat
+          (try congruence;
+           try omega;
+           try RWEvent.ltb_tac;
+           try Const.ltb_tac;
+           try Ordering.ltb_tac;
+           try ltb_des).
+    Qed.
+
+    Lemma ltb_irrefl x: ~ ltb x x.
+    Proof.
+      destruct x; simpl in *; auto;
+        repeat
+          (try congruence;
+           try omega;
+           try RWEvent.ltb_tac;
+           try Const.ltb_tac;
+           try Ordering.ltb_tac;
+           try ltb_des).
+    Qed.
+
+    Lemma ltb_eq (lhs rhs:t) (LR: ~ ltb lhs rhs) (RL: ~ ltb rhs lhs): lhs = rhs.
+    Proof.
+      destruct lhs, rhs; simpl in *; auto;
+        repeat
+          repeat
+          (try congruence;
+           try omega;
+           try RWEvent.ltb_tac;
+           try Const.ltb_tac;
+           try Ordering.ltb_tac;
+           try ltb_des).
+    Qed.
+  End Raw.
+
+  Include Raw <+ BoolOrderedType.Make (Raw).
+
+  Definition get_ordering (e:t): Ordering.t :=
+    match e with
+    | rw e _ => RWEvent.get_ordering e
+    | fence ord => ord
+    end.
+
+  Definition observable (msg:t): bool :=
+    match msg with
+    | rw e _ => if RWEvent.is_writing e then true else false
+    | fence _ => false
+    end.
+
+  Definition get_memevent (msg:t): ThreadEvent.mem_t :=
+    match msg with
+    | rw e _ => ThreadEvent.rw e
+    | fence ord => ThreadEvent.fence ord
+    end.
+End Message.
+
+Module Inception <: OrderedTypeWithLeibniz.
+  Module Raw <: BoolOrderedType.S.
+    Structure t_ := mk {
+      msg: Message.t;
+      threads: IdentSet.t;
+    }.
+    Definition t := t_.
+
+    Definition eq_dec (x y:t): {x = y} + {x <> y}.
+    Proof.
+      decide equality.
+      - destruct (IdentSet.eq_dec threads0 threads1).
+        + left. apply IdentSet.eq_leibniz. auto.
+        + right. contradict n. auto. subst. reflexivity.
+      - apply Message.eq_dec.
+    Qed.
+
+    Definition ltb (lhs rhs:t): bool :=
+      compose_comparisons [Message.compare lhs.(msg) rhs.(msg); IdentSet.compare lhs.(threads) rhs.(threads)].
+
+    Lemma ltb_trans (x y z:t) (XY: ltb x y) (YZ: ltb y z): ltb x z.
+    Proof.
+    Admitted.
+
+    Lemma ltb_irrefl x: ~ ltb x x.
+    Proof.
+    Admitted.
+
+    Lemma ltb_eq (lhs rhs:t) (LR: ~ ltb lhs rhs) (RL: ~ ltb rhs lhs): lhs = rhs.
+    Proof.
+    Admitted.
+  End Raw.
+
+  Include Raw <+ BoolOrderedType.Make (Raw).
+End Inception.
+
+Module InceptionSet := UsualSet (Inception).
+
+Module Buffer.
+  Definition t := list Message.t.
+
+  Definition empty: t := nil.
+
+  Definition timestamp (loc:Loc.t) (b:t): nat :=
+    List.fold_left
+      (fun res msg =>
+         match msg with
+         | Message.rw event timestamp =>
+           if option_eq_dec
+                Loc.eq_dec
+                (option_map fst (RWEvent.is_writing event))
+                (Some loc)
+           then max timestamp res
+           else res
+         | _ => res
+         end)
+      b
+      0.
+End Buffer.
+
+Module Memory.
+  Structure t := mk {
+    buffers: IdentMap.t Buffer.t;
+    inceptions: InceptionSet.t;
+  }.
+
+  Definition init (syntax:Program.syntax) :=
+    Memory.mk
+      (IdentMap.map (fun _ => Buffer.empty) syntax)
+      InceptionSet.empty.
+
+  Definition update_buffer (i:Ident.t) (b:Buffer.t) (m:t): t :=
+    mk (IdentMap.add i b m.(buffers)) m.(inceptions).
+
+  Definition update_inceptions (inceptions:InceptionSet.t) (m:t): t :=
+    mk m.(buffers) inceptions.
+
+  Module Position.
+    Inductive t :=
+    | init
+    | buffer (i:Ident.t) (pos:nat)
+    | inception (i:Inception.t)
+    .
+
+    Definition is_inception_of (p:t) (i:Ident.t): bool :=
+      match p with
+      | inception (Inception.mk _ threads) => IdentSet.mem i threads
+      | _ => false
+      end.
+  End Position.
+
+  Inductive In (m:t): forall (msg:Message.t) (p:Position.t), Prop :=
+  | In_init
+      loc:
+      In m (Message.rw (RWEvent.write loc Const.zero Ordering.release) 0) Position.init
+  | In_buffer
+      b msg i n
+      (BUFFER: IdentMap.find i m.(buffers) = Some b)
+      (IN: List.nth_error b n = Some msg):
+      In m msg (Position.buffer i n)
+  | In_inception
+      msg threads
+      (INCEPTION: InceptionSet.mem (Inception.mk msg threads) m.(inceptions)):
+      In m msg (Position.inception (Inception.mk msg threads))
+  .
+
+  Definition timestamp_inceptions (loc:Loc.t) (inceptions:InceptionSet.t): nat :=
+    InceptionSet.fold
+      (fun inception res =>
+         match inception with
+         | Inception.mk (Message.rw event timestamp) _ =>
+           if option_eq_dec
+                Loc.eq_dec
+                (option_map fst (RWEvent.is_writing event))
+                (Some loc)
+           then max timestamp res
+           else res
+         | _ => res
+         end)
+      inceptions
+      0.
+
+  Definition timestamp (loc:Loc.t) (m:t): nat :=
+    max (IdentMap.get_max
+           (Buffer.timestamp loc)
+           m.(buffers))
+        (timestamp_inceptions loc m.(inceptions)).
+
+  Inductive step (c:Clocks.t): forall (m1:t) (i:Ident.t) (e:ThreadEvent.mem_t) (m2:t), Prop :=
+  | step_read
+      m read_event ts position
+      i b loc val ord
+      (MESSAGE: In m (Message.rw read_event ts) position)
+      (READ: RWEvent.is_writing read_event = Some (loc, val))
+      (POSITION: ~ Position.is_inception_of position i)
+      (BUFFER: IdentMap.find i m.(buffers) = Some b)
+      (TS1: LocFun.find loc (IdentFun.find i c) <= ts)
+      (TS2: Buffer.timestamp loc b <= ts):
+      step c m i (ThreadEvent.rw (RWEvent.read loc val ord))
+           (mk (IdentMap.add i (b ++ [Message.rw (RWEvent.read loc val ord) ts]) m.(buffers)) m.(inceptions))
+  | step_write
+      m
+      i b loc val ord
+      (BUFFER: IdentMap.find i m.(buffers) = Some b):
+      step c m i (ThreadEvent.rw (RWEvent.write loc val ord))
+           (mk (IdentMap.add i (b ++ [Message.rw (RWEvent.write loc val ord) ((timestamp loc m) + 1)]) m.(buffers)) m.(inceptions))
+  | step_update
+      m read_event position
+      i b loc valr valw ord
+      (MESSAGE: In m (Message.rw read_event (timestamp loc m)) position)
+      (READ: RWEvent.is_writing read_event = Some (loc, valr))
+      (POSITION: ~ Position.is_inception_of position i)
+      (BUFFER: IdentMap.find i m.(buffers) = Some b)
+      (TS: LocFun.find loc (IdentFun.find i c) <= (timestamp loc m)):
+      step c m i (ThreadEvent.rw (RWEvent.update loc valr valw ord))
+           (mk (IdentMap.add i (b ++ [Message.rw (RWEvent.update loc valr valw ord) ((timestamp loc m) + 1)]) m.(buffers)) m.(inceptions))
+  | step_fence
+      m i b ord
+      (BUFFER: IdentMap.find i m.(buffers) = Some b):
+      step c m i (ThreadEvent.fence ord)
+           (mk (IdentMap.add i (b ++ [Message.fence ord]) m.(buffers)) m.(inceptions))
+  .
+
+  Section Consistency.
+    Variable (m:t).
+
+    Inductive prod (pred1 pred2: Message.t -> Prop): relation Position.t :=
+    | prod_intro
+        pos1 pos2 msg1 msg2
+        (POS1: In m msg1 pos1)
+        (POS2: In m msg2 pos2)
+        (MSG1: pred1 msg1)
+        (MSG2: pred2 msg2):
+        prod pred1 pred2 pos1 pos2
+    .
+
+    Inductive compose (rel1 rel2:relation Position.t): relation Position.t :=
+    | compose_intro
+        x y z
+        (REL1: rel1 x y)
+        (REL2: rel2 y z):
+        compose rel1 rel2 x z
+    .
+
+    Inductive acyclic (rel:relation Position.t): Prop :=
+    | acyclic_intro
+        (ACYCLIC: Irreflexive (tc rel))
+    .
+
+    Inductive sb: relation Position.t :=
+    | sb_init
+        i pos:
+        sb Position.init (Position.buffer i pos)
+    | sb_buffer
+        i pos1 pos2
+        (LT: pos1 < pos2):
+        sb (Position.buffer i pos1) (Position.buffer i pos2)
+    | sb_inception
+        i1 pos1 inception2
+        (INCEPTION: IdentSet.mem i1 inception2.(Inception.threads)):
+        sb (Position.buffer i1 pos1) (Position.inception inception2)
+    .
+
+    Inductive sbw: relation Position.t :=
+    | sbw_writing
+        pos1 pos2 e1 e2 ts1 ts2 loc val1 val2
+        (SB: sb pos1 pos2)
+        (POS1: In m (Message.rw e1 ts1) pos1)
+        (POS2: In m (Message.rw e2 ts2) pos2)
+        (WRITE1: RWEvent.is_writing e1 = Some (loc, val1))
+        (WRITE2: RWEvent.is_writing e2 = Some (loc, val2)):
+        sbw pos1 pos2
+    | sbw_fence
+        pos1 pos2 ord1 e2 ts2
+        (SB: sb pos1 pos2)
+        (POS1: In m (Message.fence ord1) pos1)
+        (POS2: In m (Message.rw e2 ts2) pos2):
+        sbw pos1 pos2
+    .
+
+    Inductive rfr: relation Position.t :=
+    | rfr_intro
+        write_pos read_pos
+        write_event ts
+        loc val ord
+        (WRITEPOS: In m (Message.rw write_event ts) write_pos)
+        (READPOS: In m (Message.rw (RWEvent.read loc val ord) ts) read_pos)
+        (WRITE: RWEvent.is_writing write_event = Some (loc, val)):
+        rfr write_pos read_pos
+    .
+
+    Inductive rfu: relation Position.t :=
+    | rfu_intro
+        write_pos update_pos
+        write_event ts
+        loc valr valw ord
+        (WRITEPOS: In m (Message.rw write_event ts) write_pos)
+        (UPDATEPOS: In m (Message.rw (RWEvent.update loc valr valw ord) (ts + 1)) update_pos)
+        (WRITE: RWEvent.is_writing write_event = Some (loc, valr)):
+        rfu write_pos update_pos
+    .
+
+    Definition rf: relation Position.t := rfr \2/ rfu.
+
+    Definition rseq: relation Position.t :=
+      compose
+        (rc sbw)
+        (rtc rfu).
+
+    Inductive aseq: relation Position.t :=
+    | aseq_refl
+        pos:
+        aseq pos pos
+    | aseq_fence
+        pos1 pos2 ord2
+        (SB: sb pos1 pos2)
+        (POS2: In m (Message.fence ord2) pos2):
+        aseq pos1 pos2
+    .
+
+    Definition sw: relation Position.t :=
+      (compose rseq (compose rf aseq))
+        /2\
+        (prod
+           (fun msg => Ordering.ord Ordering.release (Message.get_ordering msg))
+           (fun msg => Ordering.ord Ordering.acquire (Message.get_ordering msg)))
+    .
+
+    Definition hb: relation Position.t := tc (sb \2/ sw).
+
+    Inductive consistent: Prop :=
+    | consistent_intro
+        (CoHB: acyclic hb)
+        (CoRF: acyclic (compose hb rf))
+    .
+  End Consistency.
+End Memory.
