Makefile
@@ -16,8 +16,8 @@ Makefile.coq: Makefile $(COQTHEORIES)
    echo "-R lib/paco/src Paco"; \
    \
    echo "-R src/lib $(COQMODULE)"; \
-   echo "-R src/mem $(COQMODULE)"; \
    echo "-R src/lang $(COQMODULE)"; \
+   echo "-R src/while $(COQMODULE)"; \
    echo "-R src/sim $(COQMODULE)"; \
    echo "-R src/reorder $(COQMODULE)"; \
    \
